pulse/ulib/experimental/Steel.SelSpinLock.fst
@@ -1,0 +1,114 @@
+(*
+   Copyright 2020 Microsoft Research
+
+   Licensed under the Apache License, Version 2.0 (the "License");
+   you may not use this file except in compliance with the License.
+   You may obtain a copy of the License at
+
+       http://www.apache.org/licenses/LICENSE-2.0
+
+   Unless required by applicable law or agreed to in writing, software
+   distributed under the License is distributed on an "AS IS" BASIS,
+   WITHOUT WARRANTIES OR CONDITIONS OF ANY KIND, either express or implied.
+   See the License for the specific language governing permissions and
+   limitations under the License.
+*)
+
+module Steel.SelSpinLock
+
+open FStar.Ghost
+open Steel.SelEffect.Atomic
+open Steel.SelEffect
+open Steel.SelReference
+open Steel.FractionalPermission
+
+#set-options "--ide_id_info_off --fuel 0 --ifuel 0"
+
+let available = false
+let locked = true
+
+let lockinv (p:vprop) (r:ref bool) : vprop =
+  h_exists (fun b -> pts_to r full_perm (Ghost.hide b) `star` (if b then emp else p))
+
+let lock_t = ref bool & erased iname
+
+let protects (l:lock_t) (p:vprop) : prop = snd l >--> lockinv p (fst l)
+
+val intro_lockinv_available (#uses:inames) (p:vprop) (r:ref bool)
+  : SteelSelGhostT unit uses (pts_to r full_perm available `star` p) (fun _ -> lockinv p r)
+
+val intro_lockinv_locked (#uses:inames) (p:vprop) (r:ref bool)
+  : SteelSelGhostT unit uses (pts_to r full_perm locked) (fun _ -> lockinv p r)
+
+let intro_lockinv_available #uses p r =
+  intro_exists false
+    (fun (b: bool) ->
+      pts_to r full_perm (Ghost.hide b) `star`
+        (if b then emp else p)
+    )
+
+let intro_lockinv_locked #uses p r =
+  intro_exists true
+    (fun b -> pts_to r full_perm (Ghost.hide b) `star`
+          (if b then emp else p))
+
+let new_lock (p:vprop)
+  : SteelSelT (lock p) p (fun _ -> emp) =
+  let r = alloc_pt available in
+  intro_lockinv_available p r;
+  let i:inv (lockinv p r) = new_invariant (lockinv p r) in
+  return (r, i)
+
+val acquire_core (#p:vprop) (#u:inames) (r:ref bool) (i:inv (lockinv p r))
+  : SteelSelAtomicT bool u
+    (lockinv p r `star` emp)
+    (fun b -> lockinv p r  `star` (if b then p else emp))
+
+let acquire_core #p #u r i =
+  let ghost = witness_exists () in
+
+  let res = cas_pt r ghost available locked in
+
+  (* Not sure we can avoid calling an SMT here. Better force the manual call? *)
+  rewrite_slprop (if (Ghost.reveal ghost) then emp else p) (if res then p else emp)
+    (fun _ -> ());
+  rewrite_slprop (if res then pts_to r full_perm (Ghost.hide locked) else pts_to r full_perm ghost) (pts_to r full_perm locked) (fun _ -> ());
+
+  intro_lockinv_locked p r;
+  return res
+
+let rec acquire #p l =
+  let r:ref bool = fst l in
+  let i: inv (lockinv p r) = snd l in
+  let b = with_invariant i (fun _ -> acquire_core r i) in
+  if b then (
+    rewrite_slprop (if b then p else emp) p (fun _ -> ());
+    noop ()
+  ) else (
+    rewrite_slprop (if b then p else emp) emp (fun _ -> ());
+    acquire l
+  )
+
+val release_core (#p:vprop) (#u:inames) (r:ref bool) (i:inv (lockinv p r))
+  : SteelSelAtomicT bool u
+    (lockinv p r `star` p)
+    (fun b -> lockinv p r `star` (if b then emp else p))
+
+let release_core #p #u r i =
+  let v = witness_exists () in
+
+  let res = cas_pt r v locked available in
+
+  (* Not sure we can avoid calling an SMT here. Better force the manual call? *)
+  rewrite_slprop (if (Ghost.reveal v) then emp else p) (if res then emp else p)
+    (fun _ -> ());
+  rewrite_slprop (if res then pts_to r full_perm (Ghost.hide available) else pts_to r full_perm v) (pts_to r full_perm available) (fun _ -> ());
+
+  intro_lockinv_available p r;
+  return res
+
+let release (#p:vprop) (l:lock p) =
+  let r:ref bool = fst l in
+  let i: inv (lockinv p r) = snd l in
+  let b = with_invariant i (fun _ -> release_core r i) in
+  drop (if b then emp else p)
