pulse/ulib/experimental/Steel.SelSpinLock.fsti
@@ -1,0 +1,33 @@
+(*
+   Copyright 2020 Microsoft Research
+
+   Licensed under the Apache License, Version 2.0 (the "License");
+   you may not use this file except in compliance with the License.
+   You may obtain a copy of the License at
+
+       http://www.apache.org/licenses/LICENSE-2.0
+
+   Unless required by applicable law or agreed to in writing, software
+   distributed under the License is distributed on an "AS IS" BASIS,
+   WITHOUT WARRANTIES OR CONDITIONS OF ANY KIND, either express or implied.
+   See the License for the specific language governing permissions and
+   limitations under the License.
+*)
+
+module Steel.SelSpinLock
+open Steel.Memory
+open Steel.SelEffect
+
+val lock_t : Type u#0
+val protects (l:lock_t) (p:vprop) : prop
+
+let lock (p:vprop) = l:lock_t{l `protects` p}
+
+val new_lock (p:vprop)
+  : SteelSelT (lock p) p (fun _ -> emp)
+
+val acquire (#p:vprop) (l:lock p)
+  : SteelSelT unit emp (fun _ -> p)
+
+val release (#p:vprop) (l:lock p)
+  : SteelSelT unit p (fun _ -> emp)
